update propt with new Returns

src/coq/PropT.v
@@ -27,21 +27,34 @@ Section PropMonad.
 
   Inductive Returns {E} {A: Type} (a: A) : itree E A -> Prop :=
   | ReturnsRet: forall t, t ≈ Ret a -> Returns a t
-  | ReturnsTau: forall t, Returns a t -> Returns a (Tau t)
+  | ReturnsTau: forall t u, t ≈ Tau u -> Returns a u -> Returns a t
   | ReturnsVis: forall {X} (e: E X) (x: X) t k, t ≈ Vis e k -> Returns a (k x) -> Returns a t
   .
   Hint Constructors Returns: core.
 
+  Definition bind_PropT {E} :=
+    fun A B (PA: PropT E A) (K: A -> PropT E B) (tb: itree E B) =>
+      exists (ta: itree E A) (k: A -> itree E B),
+        PA ta /\
+        tb ≈ bind ta k /\
+        (forall a, Returns a ta -> K a (k a)).
+
+  
+  Definition bind_PropT' {E} := 
+    fun A B (PA: PropT E A) (K: A -> PropT E B) (tb: itree E B) =>
+      exists (ta: itree E A),  PA ta /\
+                          ((exists (k: A -> itree E B),
+                               (forall a, Returns a ta -> K a (k a))
+                               /\ tb ≈ bind ta k)
+                           \/ (forall k, (forall a, K a (k a)) /\ tb ≈ bind ta k)).
+    
   Global Instance Monad_Prop {E} : Monad (PropT E) :=
     {|
       ret := fun _ x y => y ≈ ret x
-      ; bind := fun A B (PA: PropT E A) (K: A -> PropT E B) (tb: itree E B) =>
-                  exists (ta: itree E A) (k: A -> itree E B),
-                    PA ta /\
-                    tb ≈ bind ta k /\
-                    (forall a, Returns a ta -> K a (k a))
+      ; bind := bind_PropT'
     |}.
 
+  
   (*
   Inductive iter_Prop {R I : Type} (step : I -> I + R -> Prop) (i : I) (r : R)
     : Prop :=
@@ -55,6 +68,7 @@ Section PropMonad.
   Polymorphic Instance MonadIter_Prop : MonadIter Ensembles.Ensemble := @iter_Prop.
   *)
 
+  (* SAZ: maybe define directly by coinduction  *)
   Global Polymorphic Instance MonadIter_Prop {E} : MonadIter (PropT E) :=
     fun R I (step : I -> PropT E (I + R)) i (r : itree E R)  =>
       exists (step': I -> itree E (I + R)%type),
@@ -77,10 +91,12 @@ Section MonadLaws.
     - revert y H. induction HRet; intros.
       constructor; rewrite <- H, H0; reflexivity.
       apply IHHRet, eqit_inv_tauL; auto.
+      rewrite <- H0. rewrite H. reflexivity.
       econstructor 3; [rewrite <- H0, H; reflexivity | apply IHHRet; reflexivity].
     - revert x H; induction HRet; intros ? EQ.
       constructor; rewrite EQ; eauto.
       apply IHHRet, eqit_inv_tauR; auto.
+      rewrite EQ. rewrite <- H. reflexivity.
       econstructor 3; [rewrite EQ, H; reflexivity | apply IHHRet; reflexivity].
   Qed.
 
@@ -98,44 +114,88 @@ Section MonadLaws.
     punfold H; inv H.
   Qed.
 
+  Lemma Returns_Ret_ : forall E A (a x : A) (t:itree E A), t ≈ Ret x -> Returns a t -> x = a.
+  Proof.
+    intros E A a x t eq H. 
+    induction H.
+    - rewrite eq in H. eapply eutt_inv_ret. apply H.
+     - rewrite tau_eutt in H. rewrite <- H in IHReturns. apply IHReturns. assumption.
+    - rewrite eq in H. apply eqit_inv_ret_vis in H. contradiction.
+  Qed.
+
+  Lemma Returns_Ret :  forall E A (a x : A), Returns a ((Ret x) : itree E A) -> x = a.
+  Proof.
+    intros.  eapply Returns_Ret_. 2: eassumption. reflexivity.
+  Qed.
+    
   Lemma ret_bind: forall {E} (a b : Type) (f : a -> PropT E b) (x : a),
       eutt_closed (f x) ->
       eqm (bind (ret x) f) (f x).
   Proof.
     intros.
     split; [| split].
-    + intros t t' eq; split; intros eqtt'.
+    - intros t t' eq; split; intros eqtt'.
       * cbn in *.
-        destruct eqtt' as (ta & k &  EQ1 & EQ2 & KA).
-        rewrite EQ1, Eq.bind_ret_l, eq in EQ2.
-        eapply H; [apply EQ2 | apply KA].
-        constructor 1; eauto.
-      * cbn.
-        exists (Ret x), (fun _ => t); split; [reflexivity | split].
-        rewrite Eq.bind_ret_l; reflexivity.
-        intros.
-        inv H0.
-        { apply eqit_inv_ret in H1; subst.
-          eapply H; eauto.
-        }
-        {
-          exfalso; eapply eutt_ret_vis_abs; eauto. }
-    + intros t t' EQ; cbn; split; intros (? & ? & ? & ? & ?).
-      * exists (Ret x), (fun _ => t'); split; [reflexivity | split; [rewrite Eq.bind_ret_l; reflexivity |]].
-        intros ? RET; inv RET.
-        2: exfalso; eapply eutt_ret_vis_abs; eauto.
-        apply eqit_inv_ret in H3; subst.
-        eapply H, H2.
-        2:rewrite H0; constructor; reflexivity.
-        rewrite H0, Eq.bind_ret_l in H1; rewrite <- EQ, H1; reflexivity.
-      * exists (Ret x), (fun _ => t); split; [reflexivity | split; [rewrite Eq.bind_ret_l; reflexivity |]].
-        intros ? RET; inv RET.
-        2: exfalso; eapply eutt_ret_vis_abs; eauto.
-        apply eqit_inv_ret in H3; subst.
-        eapply H, H2.
-        2:rewrite H0; constructor; reflexivity.
-        rewrite H0, Eq.bind_ret_l in H1; rewrite EQ, H1; reflexivity.
-    + assumption.
+        repeat red in eqtt'.
+        destruct eqtt' as (ta & EQ1 & [(k & KA & EQ2) | HX]).
+        + unfold bind, Monad_itree in EQ2. rewrite EQ1, Eq.bind_ret_l, eq in EQ2.
+          eapply H; [apply EQ2 | apply KA].
+          constructor 1; eauto.
+        + specialize (HX (fun a => t')).
+          cbn in HX. destruct HX. apply H0.
+     * cbn.
+       exists (Ret x). split; [reflexivity|].
+       left. exists (fun _ => t); split.
+        + intros.
+          apply Returns_Ret in H0. subst. red in H. rewrite eq. assumption.
+        + unfold bind, Monad_itree. rewrite Eq.bind_ret_l; reflexivity.
+          
+
+    - intros t t' EQ; cbn; split; intros HX.
+      * destruct HX as  (ta & EQ1 & [(k & KA & EQ2) | HX]).
+        + exists (Ret x); split; [reflexivity |].
+          left. exists (fun _ => t).
+          split.
+          intros ? RET; inv RET.
+          2: { rewrite tau_eutt in H0. rewrite <- H0 in H1. apply Returns_Ret in H1. subst.
+               red in H. rewrite EQ2. rewrite EQ1.
+               unfold bind, Monad_itree.
+               rewrite Eq.bind_ret_l. apply KA. rewrite EQ1. constructor. reflexivity. }
+          2: exfalso; eapply eutt_ret_vis_abs; eauto.
+          apply eqit_inv_ret in H0; subst.
+          eapply H. rewrite EQ1 in EQ2.
+          unfold bind, Monad_itree in EQ2.
+          rewrite Eq.bind_ret_l in EQ2. apply EQ2.
+          apply KA. rewrite EQ1. constructor. reflexivity.
+          unfold bind, Monad_itree.
+          rewrite Eq.bind_ret_l. rewrite EQ. reflexivity.
+          
+        + exists (Ret x); split; [reflexivity|].
+          right. intros. specialize (HX k). destruct HX. split;[ tauto | ].
+          rewrite EQ1 in H1. rewrite <- EQ. assumption.
+          
+      * destruct HX as  (ta & EQ1 & [(k & KA & EQ2) | HX]).
+        + exists (Ret x); split; [reflexivity |].
+          left. exists (fun _ => t).
+          split.
+          intros ? RET; inv RET.
+          2: { rewrite tau_eutt in H0. rewrite <- H0 in H1. apply Returns_Ret in H1. subst.
+               red in H. rewrite EQ. rewrite EQ2. rewrite EQ1. 
+               unfold bind, Monad_itree.
+               rewrite Eq.bind_ret_l. apply KA. rewrite EQ1. constructor. reflexivity. }
+          2: exfalso; eapply eutt_ret_vis_abs; eauto.
+          apply eqit_inv_ret in H0; subst.
+          eapply H. rewrite EQ1 in EQ2.
+          unfold bind, Monad_itree in EQ2.
+          rewrite Eq.bind_ret_l in EQ2. rewrite EQ. apply EQ2.
+          apply KA. rewrite EQ1. constructor. reflexivity.
+          unfold bind, Monad_itree.
+          rewrite Eq.bind_ret_l. rewrite EQ. reflexivity.
+          
+        + exists (Ret x); split; [reflexivity|].
+          right. intros. specialize (HX k). destruct HX. split;[ tauto | ].
+          rewrite EQ1 in H1. rewrite EQ. assumption.
+    - assumption.
   Qed.
 
   Section ReturnsBind.
@@ -178,7 +238,7 @@ Section MonadLaws.
         constructor; auto.
         intros u HR.
         apply REL0.
-        rewrite itree_eta, <- Heqot1; constructor 2; auto.
+        rewrite itree_eta,  <- Heqot1.  econstructor 2. reflexivity. assumption.
       - gstep. econstructor.
         intros; apply ID; unfold id.
         gbase.
@@ -192,7 +252,7 @@ Section MonadLaws.
         econstructor.
         3:{ eapply IHEQV; eauto.
             intros ? HR; apply REL.
-            rewrite itree_eta, <- Heqot1; constructor 2; eauto.
+            rewrite itree_eta, <- Heqot1; econstructor 2. reflexivity. eauto.
         }
         3,4:auto_ctrans_eq.
         2: reflexivity.
@@ -215,6 +275,69 @@ Section MonadLaws.
 
   End ReturnsBind.
 
+  Lemma distinguish_bind {E} {A B}
+        (a : A)
+        (ma : itree E A)
+        (k1 k2 : A -> itree E B)
+        (HRET : Returns a ma)
+        (NEQ: ~((k1 a) ≈ (k2 a))) : 
+    not ((ITree.bind ma k1) ≈ (ITree.bind ma k2)).
+  Proof.
+    intro HI.
+    apply NEQ. clear NEQ.
+    revert k1 k2 HI.
+    induction HRET; intros.
+    - rewrite H in HI. cbn in HI. rewrite Eq.bind_ret_l in HI. rewrite Eq.bind_ret_l in HI.
+      assumption.
+    - apply IHHRET. unfold bind, Monad_itree in HI.
+      rewrite H in HI.
+      do 2 rewrite Eq.bind_tau in HI.
+      do 2 rewrite tau_eutt in HI. apply HI.
+    - apply IHHRET. rewrite H in HI.
+      do 2 rewrite bind_vis in HI.
+      apply eqit_inv_vis in HI.
+      destruct HI as (_ & HI).
+      apply HI.
+  Qed.
+  
+
+  Lemma not_Returns {E} {A B} : inhabited B ->
+    forall (ta: itree E A), (exists tb, forall (k : A -> itree E B), tb ≈ bind ta k) -> forall (a:A), ~ Returns a ta.
+  Proof.
+    intros IB ta HX a HRet; inversion IB; clear IB.
+    revert HX.
+    induction HRet; intros (tb & HK).
+    - setoid_rewrite H in HK.
+      unfold bind, Monad_itree in HK.
+      setoid_rewrite Eq.bind_ret_l in HK.
+      pose (HK (fun _ => ret X)) as t2. cbn in t2.
+      pose (HK (fun _ => ITree.spin)) as t3. cbn in t3.
+      assert (Ret X ≈ (ITree.spin : itree E B)).
+      rewrite <- t2. rewrite <- t3. reflexivity. apply eutt_Ret_spin_abs in H0. 
+      auto.
+    - apply IHHRet.
+      exists tb. intros. 
+      specialize (HK k).
+      rewrite HK. unfold bind, Monad_itree.
+      rewrite H. 
+      rewrite bind_tau. apply tau_eutt.
+    - setoid_rewrite H in HK; clear H t.
+      pose (HK (fun _ => ret X)) as t2. cbn in t2.
+      pose (HK (fun _ => ITree.spin)) as t3. cbn in t3.
+      assert (ITree.bind (Vis e k) (fun _ : A => Ret X) ≈ ITree.bind (Vis e k) (fun _ : A => ITree.spin)).
+      rewrite <- t2. rewrite <- t3.
+      reflexivity.
+      rewrite bind_vis in H. rewrite bind_vis in H.
+      apply eqit_inv_vis in H.
+      destruct H as (_ & H).
+      specialize (H x).
+      revert H.
+      change (~((ITree.bind (k x) ( fun _ : A => Ret X)) ≈ ITree.bind (k x) (fun _ : A => ITree.spin))).
+      eapply distinguish_bind. apply HRet.
+      intro H. apply eutt_Ret_spin_abs in H. auto.
+  Qed.      
+
+  
   Lemma bind_ret: forall {E} (A : Type) (PA : PropT E A),
       eutt_closed PA ->
       eqm (bind PA (fun x => ret x)) PA.
@@ -223,25 +346,44 @@ Section MonadLaws.
     split; [| split].
     + intros t t' eq; split; intros eqtt'.
       * cbn in *.
-        destruct eqtt' as (ta & k & HPA & EQ & HRET).
-        eapply H; [symmetry; eauto | clear eq t'].
-        eapply H; [eauto | clear EQ t].
-        eapply H; eauto.
-        rewrite <- (bind_ret_r _ ta) at 2.
-        apply eqit_Returns_bind'; [reflexivity |].
-        intros.
-        rewrite (HRET r); auto.
-        reflexivity.
+        destruct eqtt' as  (ta & HPA & [(k & HRET & EQ) | HX]).
+        - eapply H; [symmetry; eauto | clear eq t'].
+          eapply H; [eauto | clear EQ t].
+          eapply H; eauto.
+          rewrite <- (bind_ret_r _ ta) at 2.
+          apply eqit_Returns_bind'; [reflexivity |].
+          intros.
+          rewrite (HRET r); auto.
+          reflexivity.
+        - specialize (HX (fun x => Ret x)). destruct HX as (_ & HX).
+          unfold bind, Monad_itree in HX. rewrite Eq.bind_ret_r in HX.
+          red in H.
+          rewrite <- eq. rewrite HX. assumption.
+          
       * cbn.
-        exists t', (fun x => Ret x); split; [auto | split; [rewrite Eq.bind_ret_r; auto |]].
+        exists t'. split; [auto|].
+        left. exists (fun x => Ret x); split.  
         intros ? ?; reflexivity.
-    + intros x y EQ; split; intros (ta & k & HPA & EQ' & HRET).
+        unfold bind, Monad_itree. rewrite Eq.bind_ret_r; auto.
+        
+    + intros x y EQ; split; intros eqtt'. 
       * cbn in *.
-        exists ta, k; split; [| split]; auto.
-        rewrite <- EQ; auto.
-      * cbn in *.
-        exists ta, k; split; [| split]; auto.
-        cbn; rewrite EQ; auto.
+        destruct eqtt' as  (ta & HPA & [(k & HRET & EQ') | HX]).        
+        - exists ta.  split; [auto|].
+          left.
+          exists k; split. auto. rewrite <- EQ; auto.
+        - exists ta.  split; [auto|].
+          right. intros. specialize (HX k). destruct HX.
+          split; auto. rewrite <- EQ. assumption.
+     * cbn in *.
+        destruct eqtt' as  (ta & HPA & [(k & HRET & EQ') | HX]).        
+        - exists ta.  split; [auto|].
+          left.
+          exists k; split. auto. rewrite EQ; auto.
+        - exists ta.  split; [auto|].
+          right. intros. specialize (HX k). destruct HX.
+          split; auto. rewrite EQ. assumption.
+
     + auto.
   Qed.
 
@@ -252,11 +394,36 @@ Section MonadLaws.
   Proof.
     intros E A B t k a b HRA HRB; induction HRA.
     - cbn; rewrite H, Eq.bind_ret_l; auto.
-    - cbn in *. rewrite (eqit_tauL true t t); [| reflexivity]; auto. 
+    - cbn in *. rewrite H. rewrite (eqit_tauL true u u); [| reflexivity]; auto. 
     - cbn in *; rewrite H, bind_vis.
       eapply (ReturnsVis b e); [reflexivity | cbn; eauto].
   Qed.
 
+  Lemma Returns_bind_inversion : forall {E A B} (t : itree E A) (k : A -> itree E B) b,
+      Returns b (bind t k) ->
+      exists a, Returns a t.
+  Proof.
+    intros E A B t k b H.
+    remember (bind t k) as t2.
+    induction H; intros.
+    - rewrite Heqt2 in H.
+      apply eutt_inv_bind_ret in H.
+      destruct H as (a & HEQ & HK).
+      exists a. rewrite HEQ. constructor. reflexivity.
+    - subst.
+      (* SAZ: TODO - pick up here *)
+  Admitted.
+      
+
+  
+  (* From Coq.Logic.ChoiceFacts *)
+Definition GuardedFunctionalChoice_on {A B} :=
+  forall P : A -> Prop, forall R : A -> B -> Prop,
+    inhabited B ->
+    (forall x : A, P x -> exists y : B, R x y) ->
+    (exists f : A->B, forall x, P x -> R x (f x)).
+Axiom guarded_choice : forall {A B}, @GuardedFunctionalChoice_on A B.
+  
   Lemma bind_bind: forall {E} (A B C : Type) (PA : PropT E A) (KB : A -> PropT E B) (KC : B -> PropT E C),
       (* eutt_closed PA -> *)
       eqm (bind (bind PA KB) KC) (bind PA (fun b => bind (KB b) KC)).
@@ -266,27 +433,50 @@ Section MonadLaws.
     split; [| split].
     + intros t t' eq; split; intros eqtt'.
       * cbn in *.
-        destruct eqtt' as (tb & kbc & (ta & kab & HPA & EQb & HRETA) & EQc & HRETB).
-        rewrite eq in EQc; clear eq t.
-        setoid_rewrite EQc; clear EQc.
-        setoid_rewrite EQb. setoid_rewrite EQb in HRETB; clear EQb tb.
-        (* ta ~a> kab a *)
-        (* (ta; kab) ~b> kbc b *)
-        exists ta.
-        exists (fun b => ITree.bind (kab b) kbc).
-        split; [| split]; auto.
-        rewrite Eq.bind_bind; reflexivity.
-        intros a HRet.
-        (* ta ~a>, hence kab a *)
-        exists (kab a), kbc.
-        split; [| split]; auto.
-        reflexivity.
-        intros; apply HRETB.
-        apply Returns_bind with a; auto.
+        red in eqtt'.
+        destruct eqtt' as (tb & HBC & [(kbc & KBC & EQc) | HX]).
+        -  destruct HBC as (ta & HTA & [(kab & KAB & EQb) | HY]).
+           -- rewrite eq in EQc; clear eq t.
+              exists ta. split; [auto|].
+              left.
+              exists (fun b => ITree.bind (kab b) kbc).              
+              setoid_rewrite EQc; clear EQc.
+              setoid_rewrite EQb. setoid_rewrite EQb in KBC; clear EQb tb.
+              (* ta ~a> kab a *)
+              (* (ta; kab) ~b> kbc b *)
+              split.
+              ++ intros a HRet.
+                 exists (kab a). split.
+                 ** apply KAB; auto.
+                 ** left.
+                    exists kbc. split.
+                    intros a' HRET'. apply KBC. apply Returns_bind with a; auto.
+                    reflexivity.
+              ++ unfold bind, Monad_itree.
+                 rewrite Eq.bind_bind. reflexivity.
+           -- (* ta diverges *)
+             rewrite eq in EQc; clear eq t.
+             red.
+             exists ta. split; [auto|].
+              right.
+              setoid_rewrite EQc; clear EQc.
+              intros. split.
+             ++ intros a. red.
+                exists (bind ta (fun _ => ITree.spin)).
+                split.
+                2 : { left. exists kbc. split. intros.
+                      assert (~Returns a0 (bind ta (fun _ : A => ITree.spin))).
+                      eapply not_Returns.
+                      admit.
+                (* CONTINUE HERE: USE not_returns? *)
+                exists tb.
+                admit.
+                admit.
+                admit. }
+                admit.
+             ++ admit.
+        - admit.
       * cbn in *.
-        destruct eqtt' as (ta & kac & HPA & EQa & HRet).
-        rewrite <- eq in EQa; clear eq t'.
-        setoid_rewrite EQa; clear EQa t.
   (* ta: itree E A  (part 1)
            kac: A -> itree E C (part 2 3)
    *)
@@ -302,11 +492,15 @@ Section MonadLaws.
   (*     (forall x y, x ≈ y -> (PA x <-> PA' y)) /\ *)
   (*     eutt_closed PA /\ eutt_closed PA'. *)
 
-
   Lemma bind_bind: forall {E} (A B C : Type) (PA : PropT E A) (KB : A -> PropT E B) (KC : B -> PropT E C),
       (* eutt_closed PA -> *)
       forall x y, x ≈ y -> bind (bind PA KB) KC x -> bind PA (fun b => bind (KB b) KC) y.
   Proof.
+      (*
+    SAZ: This version depends on the old definition of bind.
+   *)
+  Admitted.
+  (*
     (* PA ~a> KB a ~b> KC b *)
     intros.
     cbn in *.
@@ -328,6 +522,7 @@ Section MonadLaws.
     intros; apply HRETB.
     apply Returns_bind with a; auto.
   Qed.
+*)
 
 End MonadLaws.
 
@@ -342,13 +537,15 @@ From ITree Require Import
 Section IterLaws.
 
   Global Instance IterUnfold_PropT {E} : IterUnfold (Kleisli (PropT E)) sum.
-  intros A B f a.
-  unfold iter, Iter_Kleisli, Basics.iter, MonadIter_Prop.
+  intros A B Pstep a.
+
   repeat red. split.
   - intros t1 t2 EQ.
     split.
     + intros (step & H & EQ2).
       cbn.
+      admit.
+(* SAZ OLD 
       exists (step a). exists (fun ab : A + B => match ab with
                                     | inl a => Tau (ITree.iter step a)
                                     | inr b => Ret b
@@ -362,26 +559,46 @@ Section IterLaws.
         destruct a0. cbn.
         exists step. split. assumption. apply Eq.eqit_tauR. reflexivity.
         cbn. reflexivity.
-    + intros H.
+*)
+    + intros H. admit.
+(* SAZ OLD       
       cbn in H.
-      destruct H as (ta & k & HF & Heq & Hbody).
+      destruct H as (ta & k & HP & EQ2 & HK).
+      unfold iter, Iter_Kleisli, Basics.iter, MonadIter_Prop.
+      exists (fun a => ITree.bind (ITree.bind ta k) (fun b => ret (inr b))).
+      split.
+      intros. specialize (HK (inl j)).
+      cbn in HK.
+      
+      (iter step') a = (cat step' (case_ (iter step') (id_ b))) a
+      
+      
+      
       specialize (Hbody (inl a)).
       cbn in Hbody.
-      (* SAZ: need to decide about Returns (inl a) ta vs. not (Returns (inl a) ta) *)
-      admit.
+      (* SAZ: need to decide about Returns (inl a) ta vs. not (Returns (inl a) ta) *)      
+      assert ((Returns (inl a) ta) \/ ~(Returns (inl a) ta)) as CLASSICAL.
+      { admit. (* TODO: Classical logic *) }
+      destruct CLASSICAL as [HRet | HNoRet].
+      apply Hbody in HRet.
+      destruct HRet as (step' & Hfj & HI).
+      exists step'. split. assumption.
+ *)
+      
   - split.
     + split; intros.
       destruct H0 as (step & Hstep & EQ).
       exists step. split; auto. rewrite EQ. assumption.
       destruct H0 as (step & Hstep & EQ).
       exists step. split; auto. rewrite EQ. symmetry. assumption.
-    + cbn.  split; intros H1.
-      * destruct H1 as (ta & k & HF & EQ & HR).
+    + cbn. admit.
+        (* old destruct H1 as (ta & k & HF & EQ & HR).
+      *
         exists ta. exists k. split; auto. split. rewrite <- EQ. symmetry. assumption.
         assumption.
       * destruct H1 as (ta & k & HF & EQ & HR).
         exists ta. exists k. split; auto. split. rewrite <- EQ. assumption.
-        assumption.
+        assumption. *)
   Admitted.
 
   Global Instance IterNatural_PropT {E} : IterNatural (Kleisli (PropT E)) sum.
@@ -390,6 +607,8 @@ Section IterLaws.
   split.
   - intros t1 t2 EQ.
     split.
+  Admitted.
+(*  
     + intros (tb & k & H & EQ2 & Hk).
       repeat red in H. destruct H as (step & Hstep & EQ3).
       repeat red. exists (fun a => bind (step a) (fun ab : A + B => match ab with
@@ -418,7 +637,7 @@ Section IterLaws.
         (* SAZ: eventually need to use: iter_natural. *)
         unfold iter, Iter_Kleisli, Basics.iter, MonadIter_itree. rewrite unfold_iter.
   Admitted.
-              
+  *)            
       
   Global Instance IterDinatural_PropT {E} : IterDinatural (Kleisli (PropT E)) sum.
   Admitted.
